\documentclass[11pt]{article}
\usepackage{setspace}
\setstretch{1}
\usepackage{amsmath,amssymb, amsthm}
\usepackage{graphicx}
\usepackage{bm}
\usepackage[hang, flushmargin]{footmisc}
\usepackage[colorlinks=true]{hyperref}
\usepackage[nameinlink]{cleveref}
\usepackage{footnotebackref}
\usepackage{url}
\usepackage{listings}
\usepackage[most]{tcolorbox}
\usepackage{inconsolata}
\usepackage[papersize={8.5in,11in}, margin=1in]{geometry}
\usepackage{float}
\usepackage{caption}
\usepackage{esint}
\usepackage{url}
\usepackage{enumitem}
\usepackage{subfig}
\usepackage{wasysym}
\newcommand{\ilc}{\texttt}
\usepackage{etoolbox}
\usepackage{algorithm}
\usepackage{changepage}
% \usepackage{algorithmic}
\usepackage[noend]{algpseudocode}
\usepackage{tikz}
\usepackage{pifont}
\usepackage{gensymb}
\usetikzlibrary{matrix,positioning,arrows.meta,arrows}
\patchcmd{\thebibliography}{\section*{\refname}}{}{}{}
% \PassOptionsToPackage{hyphens}{url}\usepackage{hyperref}

\providecommand{\myceil}[1]{\left \lceil #1 \right \rceil }
\providecommand{\myfloor}[1]{\left \lfloor #1 \right \rfloor }
\providecommand{\qbm}[1]{\begin{bmatrix} #1 \end{bmatrix}}
\providecommand{\qpm}[1]{\begin{pmatrix} #1 \end{pmatrix}}
\providecommand{\norm}[1]{\left\lVert #1 \right\rVert}
\providecommand{\len}[1]{\left| #1 \right|}
\newcommand{\cmark}{\ding{51}}%
\newcommand{\xmark}{\ding{55}}%

\begin{document}



\title{\textbf{MATH 307: Individual Homework 12}}


\author{Shaochen (Henry) ZHONG, \ilc{sxz517@case.edu}}

\date{Due and submitted on 03/22/2021 \\ Spring 2021, Dr. Guo}
\maketitle



\subsection*{Problem 1}
\textit{See HW instruction.}\newline

For $A = \qbm{1 & i \\ 1 & -i}$, we have:

\begin{align*}
    B = A^{-1} &= \qbm{1 & i \\ 1 & -i}^{-1} = \frac{1}{-2i} \qbm{-i & -i \\ -1 & 1} = \qbm{\frac{1}{2} & \frac{1}{2} \\ -\frac{1}{2}i & \frac{1}{2}i}
\end{align*}

Now to confirm that $AB = BA = I$:

\begin{align*}
    AB &= \qbm{1 & i \\ 1 & -i} \cdot \qbm{\frac{1}{2} & \frac{1}{2} \\ -\frac{1}{2}i & \frac{1}{2}i} \\
    &= \qbm{\frac{1}{2} + \frac{1}{2} & \frac{1}{2} - \frac{1}{2} \\ \frac{1}{2} - \frac{1}{2} & \frac{1}{2} + \frac{1}{2}} = \qbm{1 & 0 \\ 0 & 1} = I \\
    BA &= \qbm{\frac{1}{2} & \frac{1}{2} \\ -\frac{1}{2}i & \frac{1}{2}i} \cdot \qbm{1 & i \\ 1 & -i} \\
    &= \qbm{\frac{1}{2} + \frac{1}{2} & \frac{1}{2}i - \frac{1}{2}i \\ -\frac{1}{2}i + \frac{1}{2}i & \frac{1}{2} + \frac{1}{2}} = \qbm{1 & 0 \\ 0 & 1} = I \\
\end{align*}


\subsection*{Problem 2}
\textit{See HW instruction.}\newline

\subsubsection*{(a)}

Let $x = \qbm{x_1 \\ x_2}$, we have:

\begin{align*}
    Ax &= \qbm{\frac{\sqrt{2}}{2} & -\frac{\sqrt{2}}{2} \\ \frac{\sqrt{2}}{2} & \frac{\sqrt{2}}{2}} \cdot \qbm{x_1 \\ x_2} = b = \qbm{0 \\ 2 \sqrt{2}} \\
    &= \begin{cases}
        \frac{\sqrt{2}}{2} x_1 -\frac{\sqrt{2}}{2} x_2 = 0 \\
        \frac{\sqrt{2}}{2} x_1 +\frac{\sqrt{2}}{2} x_2 = 2 \sqrt{2}
    \end{cases} = \begin{cases}
        x_1 = 2 \\
        x_2 = 2
    \end{cases} \\
    \Longrightarrow x &= \qbm{2 \\ 2}
\end{align*}

\subsubsection*{(b)}
If $A$ is to rotate $x$ for $45 \degree$ to $b$, reversely, we may counter rotate $b$ $-45 \degree$ to get $x$. As we have shown in \textit{Group HW5} and \textit{Group HW6}, to rotate a vector for $\phi$ degree, we need to left multiply $\qbm{\cos \phi & -\sin \phi \\ \sin \phi & \cos \phi}$ to the target vector.

In this case, we have $\phi$ to be $-\frac{\pi}{4}$, thus the rotation matrix should be $\qbm{\frac{\sqrt{2}}{2} & \frac{\sqrt{2}}{2} \\ -\frac{\sqrt{2}}{2} & \frac{\sqrt{2}}{2}}$. We call this matrix $C$ and now we try to left multiply it with $b$ to get $x$:

\begin{align*}
    C b &= \qbm{\frac{\sqrt{2}}{2} & \frac{\sqrt{2}}{2} \\ -\frac{\sqrt{2}}{2} & \frac{\sqrt{2}}{2}} \cdot \qbm{0 \\ 2 \sqrt{2}} = x\\
    x &= \qbm{2 \\ 2}
\end{align*}

\subsubsection*{(c)}

We know $A$ is an orthogonal matrix as:

\begin{equation*}
    A A^{T} =  \qbm{\frac{\sqrt{2}}{2} & -\frac{\sqrt{2}}{2} \\ \frac{\sqrt{2}}{2} & \frac{\sqrt{2}}{2}}  \cdot \qbm{\frac{\sqrt{2}}{2} & \frac{\sqrt{2}}{2} \\ -\frac{\sqrt{2}}{2} & \frac{\sqrt{2}}{2}} = \qbm{\frac{1}{2} + \frac{1}{2} & \frac{1}{2} - \frac{1}{2} \\ \frac{1}{2} - \frac{1}{2} & \frac{1}{2} + \frac{1}{2}} = \qbm{1 & 0 \\ 0 & 1} = I
\end{equation*}

Known this, we also know that $A^{-1} = A^T = \qbm{\frac{\sqrt{2}}{2} & \frac{\sqrt{2}}{2} \\ -\frac{\sqrt{2}}{2} & \frac{\sqrt{2}}{2}}$. Now we may left multiply $A^{-1}$ to the both sides of $Ax = b$:

\begin{align*}
    A^{-1} A x &= A^{-1} b \\
    I x &= A^{-1} b \\
    x &= \qbm{\frac{\sqrt{2}}{2} & \frac{\sqrt{2}}{2} \\ -\frac{\sqrt{2}}{2} & \frac{\sqrt{2}}{2}} \cdot \qbm{0 \\ 2 \sqrt{2}} = \qbm{2 \\ 2}
\end{align*}

\end{document}

